src/QUIC.Impl.fsti
@@ -1,22 +1,31 @@
 /// An implementation of QUIC.Spec.fst that is concerned only with functional
-/// correctness (no notion of model for now).
+/// correctness and side-channel resistance (no notion of model for now).
 module QUIC.Impl
 include QUIC.Impl.Crypto
 include QUIC.Impl.Header.Base
 
 module Spec = QUIC.Spec
-module QImpl = QUIC.Impl.Header.Base
 module PN = QUIC.Spec.PacketNumber.Base
 module Secret = QUIC.Secret.Int
 module Seq = QUIC.Secret.Seq
+module Parse = QUIC.Spec.Header.Parse
 
 // This MUST be kept in sync with QUIC.Impl.fst...
 module G = FStar.Ghost
 module B = LowStar.Buffer
 module S = FStar.Seq
 module HS = FStar.HyperStack
-module ST = FStar.HyperStack.ST
+module HST = FStar.HyperStack.ST
 
+
+module Cipher = EverCrypt.Cipher
+module AEAD = EverCrypt.AEAD
+module HKDF = EverCrypt.HKDF
+module CTR = EverCrypt.CTR
+
+module SAEAD = Spec.Agile.AEAD
+module SCipher = Spec.Agile.Cipher
+module SHKDF = Spec.Agile.HKDF
 
 module U64 = FStar.UInt64
 module U32 = FStar.UInt32
@@ -28,11 +37,7 @@ open FStar.HyperStack.ST
 open EverCrypt.Helpers
 open EverCrypt.Error
 
-#set-options "--max_fuel 0 --max_ifuel 0"
-// ... up to here!
-
-unfold noextract
-let lbytes = QUIC.Spec.Base.lbytes
+#set-options "--z3rlimit 16"
 
 /// Low-level types used in this API
 /// --------------------------------
@@ -41,203 +46,189 @@ type u2 = n:U8.t{U8.v n < 4}
 type u4 = n:U8.t{U8.v n < 16}
 type u62 = n:UInt64.t{UInt64.v n < pow2 62}
 
-#restart-solver
-
-(* Useful shortcuts *)
-
-let derive_k
-  (i: index)
-  (s: state i)
-  (h: HS.mem)
-: GTot (Seq.seq Secret.uint8)
-=
-  let s0 = g_traffic_secret (B.deref h s) in
-  Spec.derive_secret i.hash_alg s0 Spec.label_key (Spec.Agile.AEAD.key_length i.aead_alg)
-
-let derive_iv
-  (i: index)
-  (s: state i)
-  (h: HS.mem)
-: GTot (Seq.seq Secret.uint8)
-= let s0 = g_traffic_secret (B.deref h s) in
-  Spec.derive_secret i.hash_alg s0 Spec.label_iv 12
-
-let derive_pne
-  (i: index)
-  (s: state i)
-  (h: HS.mem)
-: GTot (Seq.seq Secret.uint8)
-= let s0 = g_traffic_secret (B.deref h s) in
-  Spec.derive_secret i.hash_alg s0 Spec.label_hp (ae_keysize i.aead_alg)
-
-
-val encrypt: #i:G.erased index -> (
-  let i = G.reveal i in
-  s: state i ->
-  dst: B.buffer U8.t ->
-  dst_pn: B.pointer PN.packet_number_t ->
-  h: header ->
-  plain: B.buffer Secret.uint8 ->
-  plain_len: U32.t ->
-  Stack error_code
-    (requires fun h0 ->
-      // Memory & preservation
-      B.live h0 plain /\ B.live h0 dst /\ B.live h0 dst_pn /\
-      header_live h h0 /\
-      B.(all_disjoint [ footprint h0 s; loc_buffer dst; loc_buffer dst_pn; header_footprint h; loc_buffer plain ]) /\
-      invariant h0 s /\
-      incrementable s h0 /\
-      B.length plain == U32.v plain_len /\ (
-      let clen = if is_retry h then 0 else U32.v plain_len + Spec.Agile.AEAD.tag_length i.aead_alg in
-      (if is_retry h then U32.v plain_len == 0 else 3 <= U32.v plain_len /\ U32.v plain_len < Spec.max_plain_length) /\
-      (has_payload_length h ==> Secret.v (payload_length h) == clen) /\
-      B.length dst == Secret.v (header_len h) + clen
-    ))
-    (ensures fun h0 r h1 ->
-      match r with
-      | Success ->
-          // Memory & preservation
-          B.(modifies (footprint_s h0 (deref h0 s) `loc_union` loc_buffer dst `loc_union` loc_buffer dst_pn)) h0 h1 /\
-          invariant h1 s /\
-          footprint_s h1 (B.deref h1 s) == footprint_s h0 (B.deref h0 s) /\ (
-          // Functional correctness
-          let k = derive_k i s h0 in
-          let iv = derive_iv i s h0 in
-          let pne = derive_pne i s h0 in
-          let plain = B.as_seq h0 plain in
-          let packet: packet = B.as_seq h1 dst in
-          let pn = g_last_packet_number (B.deref h0 s) h0 `Secret.add` Secret.to_u64 1uL in
-          B.deref h1 dst_pn == pn /\
-          packet == Spec.encrypt i.aead_alg k iv pne (g_header h h0 pn) (Seq.seq_reveal plain) /\
-          g_last_packet_number (B.deref h1 s) h1 == pn)
-      | _ ->
-          False))
-
-// Callers allocate this type prior to calling decrypt. The contents are only
-// meaningful, and plain is only non-null, if the decryption was a success.
-noeq
-type result = {
-  pn: PN.packet_number_t;
-  header: header;
-  header_len: Secret.uint32;
-  plain_len: Secret.uint32;
-  total_len: Secret.uint32; (* NOTE: this DOES include the tag *)
-}
-
-val initial_secrets (dst_client: B.buffer Secret.uint8)
-  (dst_server: B.buffer Secret.uint8)
-  (cid: B.buffer Secret.uint8)
-  (cid_len: U32.t):
-  Stack unit
-    (requires (fun h0 ->
-      B.(all_live h0 [ buf dst_client; buf dst_server; buf cid ]) /\
-      B.length dst_client = Spec.Agile.Hash.(hash_length SHA2_256) /\
-      B.length dst_server = Spec.Agile.Hash.(hash_length SHA2_256) /\
-      B.length cid = U32.v cid_len /\
-      U32.v cid_len <= 20 /\
-      B.(all_disjoint [ loc_buffer dst_client; loc_buffer dst_server; loc_buffer cid ])))
-    (ensures (fun h0 _ h1 ->
-      B.(modifies (loc_buffer dst_client `loc_union` loc_buffer dst_server) h0 h1)))
+val dummy: unit
 
 unfold
-let decrypt_post (i: index)
-  (s:state i)
-  (dst: B.pointer result)
-  (packet: B.buffer U8.t)
-  (len: U32.t)
-  (cid_len: U8.t)
-  (h0: HS.mem)
-  (res: error_code)
-  (h1: HS.mem): Pure Type0
-  (requires
-    U8.v cid_len <= 20 /\
-    U32.v len == B.length packet /\
-    invariant h0 s /\
-    incrementable s h0)
-  (ensures fun _ -> True)
+let encrypt_pre
+  (a: ea)
+  (aead: AEAD.state a)
+  (siv: B.buffer Secret.uint8)
+  (ctr: CTR.state (SAEAD.cipher_alg_of_supported_alg a))
+  (hpk: B.buffer Secret.uint8)
+  (dst: B.buffer U8.t)
+  (h: header)
+  (pn: PN.packet_number_t)
+  (plain: B.buffer Secret.uint8)
+  (plain_len: Secret.uint32) // should be secret, because otherwise one can compute the packet number length
+  (m: HS.mem)
+: GTot Type0
 =
-  let max (x y: nat) : Tot nat = if x >= y then x else y in
-  let k = derive_k i s h0 in
-  let iv = derive_iv i s h0 in
-  let pne = derive_pne i s h0 in
-  let prev = g_last_packet_number (B.deref h0 s) h0 in
-  invariant h1 s /\
-  footprint_s h1 (B.deref h1 s) == footprint_s h0 (B.deref h0 s) /\
+  let a' = SAEAD.cipher_alg_of_supported_alg a in
+  B.all_disjoint [
+    AEAD.footprint m aead;
+    B.loc_buffer siv;
+    CTR.footprint m ctr;
+    B.loc_buffer hpk;
+    B.loc_buffer dst;
+    header_footprint h;
+    B.loc_buffer plain;
+  ] /\
+  AEAD.invariant m aead /\
+  B.live m siv /\ B.length siv == 12 /\
+  CTR.invariant m ctr /\
+  B.live m hpk /\ B.length hpk == SCipher.key_length a' /\
+  B.live m dst /\
+  header_live h m /\
+  B.live m plain /\ B.length plain == Secret.v plain_len /\
   begin
-    let r = B.deref h1 dst in
-    match res with
-    | Success ->
-      // prev is known to be >= g_initial_packet_number (see lemma invariant_packet_number)
-      Secret.v (g_last_packet_number (B.deref h1 s) h1) == max (Secret.v prev) (Secret.v r.pn) /\ (
-
-      // Lengths
-      r.header_len == header_len r.header /\
-      Secret.v r.header_len + Secret.v r.plain_len <= Secret.v r.total_len /\
-      Secret.v r.total_len <= B.length packet /\
-      B.(loc_includes (loc_buffer (B.gsub packet 0ul (Secret.reveal r.header_len))) (header_footprint r.header)) /\
-      header_live r.header h1 /\
-      Secret.v r.total_len <= B.length packet /\
-      
-      // Contents
-      (
-      let fmt = B.as_seq h1 (B.gsub packet 0ul (Secret.reveal r.header_len)) in
-      let plain =
-        B.as_seq h1 (B.gsub packet (Secret.reveal r.header_len) (Secret.reveal r.plain_len)) in
-      let rem = B.as_seq h0 (B.gsub packet (Secret.reveal r.total_len) (B.len packet `U32.sub `Secret.reveal r.total_len)) in
-      match Spec.decrypt i.aead_alg k iv pne (Secret.v prev) (U8.v cid_len) (B.as_seq h0 packet) with
-      | Spec.Success h' plain' rem' ->
-        h' == g_header r.header h1 r.pn /\
-        fmt == QUIC.Spec.Header.Parse.format_header h' /\
-        plain' == plain /\
-        rem' == rem
-      | _ -> False
-    ))
-    | DecodeError ->
-      Spec.Failure? (Spec.decrypt i.aead_alg k iv pne (Secret.v prev) (U8.v cid_len) (B.as_seq h0 packet))
-    | AuthenticationFailure ->
-      Spec.Failure? (Spec.decrypt i.aead_alg k iv pne (Secret.v prev) (U8.v cid_len) (B.as_seq h0 packet)) /\
-      Secret.v r.total_len <= B.length packet
-    | _ ->
-      False
+    if is_retry h
+    then
+      B.length plain == 0 /\
+      B.length dst == Secret.v (header_len h)
+    else
+      B.length dst == Secret.v (header_len h) + Secret.v plain_len + SAEAD.tag_length a /\
+      3 <= Secret.v plain_len /\ Secret.v plain_len < max_plain_length
   end
 
-val decrypt: #i:G.erased index -> (
-  let i = G.reveal i in
-  s:state i ->
-  dst: B.pointer result ->
-  packet: B.buffer U8.t ->
-  len: U32.t{
-    B.length packet == U32.v len
-  } ->
-  cid_len: U8.t { U8.v cid_len <= 20 } ->
-  Stack error_code
-    (requires fun h0 ->
-      // We require clients to allocate space for a result, e.g.
-      //   result r = { 0 };
-      //   decrypt(s, &r, ...);
-      // This means that we don't require that the pointers inside ``r`` be live
-      // (i.e. NO ``header_live header`` precondition).
-      // After a successful call to decrypt, ``packet`` contains the decrypted
-      // data; ``header`` is modified to point within the header area of
-      // ``packet``; and the plaintext is within ``packet`` in range
-      // ``[header_len, header_len + plain_len)``.
-      B.live h0 packet /\ B.live h0 dst /\
-      B.(all_disjoint [ loc_buffer dst; loc_buffer packet; footprint h0 s ]) /\
-      invariant h0 s /\
-      incrementable s h0)
-    (ensures fun h0 res h1 ->
-      let r = B.deref h1 dst in
-      decrypt_post i s dst packet len cid_len h0 res h1 /\
-      begin match res with
-      | Success ->
-      B.(modifies (footprint_s h0 (deref h0 s) `loc_union`
-        loc_buffer (gsub packet 0ul (Secret.reveal r.total_len)) `loc_union` loc_buffer dst) h0 h1)
-      | DecodeError ->
-        B.modifies B.loc_none h0 h1
-      | AuthenticationFailure ->
-        B.(modifies (footprint_s h0 (deref h0 s) `loc_union`
-        loc_buffer (gsub packet 0ul (Secret.reveal r.total_len)) `loc_union` loc_buffer dst) h0 h1)
-      | _ -> False
-      end
+unfold
+let encrypt_post
+  (a: ea)
+  (aead: AEAD.state a)
+  (siv: B.buffer Secret.uint8)
+  (ctr: CTR.state (SAEAD.cipher_alg_of_supported_alg a))
+  (hpk: B.buffer Secret.uint8)
+  (dst: B.buffer U8.t)
+  (h: header)
+  (pn: PN.packet_number_t)
+  (plain: B.buffer Secret.uint8)
+  (plain_len: Secret.uint32)
+  (m: HS.mem)
+  (res: error_code)
+  (m' : HS.mem)
+: GTot Type0
+=
+  encrypt_pre a aead siv ctr hpk dst h pn plain plain_len m /\
+  B.modifies (B.loc_buffer dst `B.loc_union` AEAD.footprint m aead `B.loc_union` CTR.footprint m ctr) m m' /\
+  AEAD.invariant m' aead /\ AEAD.footprint m' aead == AEAD.footprint m aead /\
+  AEAD.preserves_freeable aead m m' /\
+  AEAD.as_kv (B.deref m' aead) == AEAD.as_kv (B.deref m aead) /\
+  CTR.invariant m' ctr /\ CTR.footprint m' ctr == CTR.footprint m ctr /\
+  B.as_seq m' dst `Seq.equal` Spec.encrypt a (AEAD.as_kv (B.deref m aead)) (B.as_seq m siv) (B.as_seq m hpk) (g_header h m pn) (Seq.seq_reveal (B.as_seq m plain)) /\
+  res == Success
+
+val encrypt
+  (a: ea)
+  (aead: AEAD.state a)
+  (siv: B.buffer Secret.uint8)
+  (ctr: CTR.state (SAEAD.cipher_alg_of_supported_alg a))
+  (hpk: B.buffer Secret.uint8)
+  (dst: B.buffer U8.t)
+  (h: header)
+  (pn: PN.packet_number_t)
+  (plain: B.buffer Secret.uint8)
+  (plain_len: Secret.uint32)
+: HST.Stack error_code
+  (requires (fun m ->
+    encrypt_pre a aead siv ctr hpk dst h pn plain plain_len m
+  ))
+  (ensures (fun m res m' ->
+    encrypt_post a aead siv ctr hpk dst h pn plain plain_len m res m'
+  ))
+
+unfold
+let decrypt_pre
+  (a: ea)
+  (aead: AEAD.state a)
+  (siv: B.buffer Secret.uint8)
+  (ctr: CTR.state (SAEAD.cipher_alg_of_supported_alg a))
+  (hpk: B.buffer Secret.uint8)
+  (dst: B.buffer U8.t)
+  (dst_len: U32.t)
+  (dst_hdr: B.pointer result)
+  (last_pn: PN.last_packet_number_t)
+  (cid_len: short_dcid_len_t)
+  (m: HS.mem)
+: GTot Type0
+=
+  let a' = SAEAD.cipher_alg_of_supported_alg a in
+  B.all_disjoint [
+    AEAD.footprint m aead;
+    B.loc_buffer siv;
+    CTR.footprint m ctr;
+    B.loc_buffer hpk;
+    B.loc_buffer dst;
+    B.loc_buffer dst_hdr;
+  ] /\
+  AEAD.invariant m aead /\
+  B.live m siv /\ B.length siv == 12 /\
+  CTR.invariant m ctr /\
+  B.live m hpk /\ B.length hpk == SCipher.key_length a' /\
+  B.live m dst /\ B.length dst == U32.v dst_len /\
+  B.live m dst_hdr
+
+unfold
+let decrypt_post
+  (a: ea)
+  (aead: AEAD.state a)
+  (siv: B.buffer Secret.uint8)
+  (ctr: CTR.state (SAEAD.cipher_alg_of_supported_alg a))
+  (hpk: B.buffer Secret.uint8)
+  (dst: B.buffer U8.t)
+  (dst_len: U32.t)
+  (dst_hdr: B.pointer result)
+  (last_pn: PN.last_packet_number_t)
+  (cid_len: short_dcid_len_t)
+  (m: HS.mem)
+  (res: error_code)
+  (m' : HS.mem)
+: GTot Type0
+=
+  decrypt_pre a aead siv ctr hpk dst dst_len dst_hdr last_pn cid_len m /\
+  AEAD.invariant m' aead /\ AEAD.footprint m' aead == AEAD.footprint m aead /\
+  AEAD.preserves_freeable aead m m' /\
+  AEAD.as_kv (B.deref m' aead) == AEAD.as_kv (B.deref m aead) /\
+  CTR.invariant m' ctr /\ CTR.footprint m' ctr == CTR.footprint m ctr /\
+  begin match res, Spec.decrypt a (AEAD.as_kv (B.deref m aead)) (B.as_seq m siv) (B.as_seq m hpk) (Secret.v last_pn) (U32.v cid_len) (B.as_seq m dst) with
+  | AuthenticationFailure, Spec.Failure ->
+    let r = B.deref m' dst_hdr in
+    Secret.v r.total_len <= B.length dst /\
+    B.modifies (AEAD.footprint m aead `B.loc_union` CTR.footprint m ctr `B.loc_union` B.loc_buffer dst_hdr `B.loc_union` B.loc_buffer (B.gsub dst 0ul (Secret.reveal r.total_len))) m m'
+  | DecodeError, Spec.Failure ->
+    B.modifies B.loc_none m m'
+  | Success, Spec.Success gh plain rem ->
+    let r = B.deref m' dst_hdr in
+    let h = r.header in
+    header_live h m' /\
+    gh == g_header h m' r.pn /\
+    r.header_len == header_len h /\
+    Secret.v r.plain_len == Seq.length plain /\
+    Secret.v r.header_len + Secret.v r.plain_len <= Secret.v r.total_len /\
+    Secret.v r.total_len <= B.length dst /\
+    B.loc_buffer (B.gsub dst 0ul (public_header_len h)) `B.loc_includes` header_footprint h /\
+    (
+      B.modifies (AEAD.footprint m aead `B.loc_union` CTR.footprint m ctr `B.loc_union` B.loc_buffer dst_hdr `B.loc_union` B.loc_buffer (B.gsub dst 0ul (Secret.reveal r.total_len))) m m' /\
+      B.as_seq m' (B.gsub dst 0ul (Secret.reveal r.header_len)) `Seq.equal` Parse.format_header (g_header h m' r.pn) /\
+      B.as_seq m' (B.gsub dst (Secret.reveal r.header_len) (Secret.reveal r.plain_len)) `Seq.equal` plain /\
+      B.as_seq m' (B.gsub dst (Secret.reveal r.total_len) (B.len dst `U32.sub` Secret.reveal r.total_len)) `Seq.equal` rem
     )
-  )
+  | _ -> False
+  end
+
+val decrypt
+  (a: ea)
+  (aead: AEAD.state a)
+  (siv: B.buffer Secret.uint8)
+  (ctr: CTR.state (SAEAD.cipher_alg_of_supported_alg a))
+  (hpk: B.buffer Secret.uint8)
+  (dst: B.buffer U8.t)
+  (dst_len: U32.t)
+  (dst_hdr: B.pointer result)
+  (last_pn: PN.last_packet_number_t)
+  (cid_len: short_dcid_len_t)
+: HST.Stack error_code
+  (requires (fun m ->
+    decrypt_pre a aead siv ctr hpk dst dst_len dst_hdr last_pn cid_len m
+  ))
+  (ensures (fun m res m' ->
+    decrypt_post a aead siv ctr hpk dst dst_len dst_hdr last_pn cid_len m res m'
+  ))
