src/QUIC.fst
@@ -1,0 +1,496 @@
+module QUIC
+
+module Cipher = EverCrypt.Cipher
+module AEAD = EverCrypt.AEAD
+module HKDF = EverCrypt.HKDF
+module CTR = EverCrypt.CTR
+module IB = LowStar.ImmutableBuffer
+module U32 = FStar.UInt32
+
+module Seq = QUIC.Secret.Seq
+module SecretBuffer = QUIC.Secret.Buffer
+
+module SHKDF = Spec.Agile.HKDF
+module SHD = Spec.Hash.Definitions
+
+open LowStar.BufferOps (* for the !* notation *)
+
+module Spec = QUIC.Spec
+module Impl = QUIC.Impl
+module Lemmas = QUIC.Impl.Lemmas
+
+
+/// Helpers
+/// -------
+
+let key_len (a: ea): x:U8.t { U8.v x = Spec.Agile.AEAD.key_length a } =
+  let open Spec.Agile.AEAD in
+  match a with
+  | AES128_GCM -> 16uy
+  | AES256_GCM -> 32uy
+  | CHACHA20_POLY1305 -> 32uy
+
+let key_len32 a = FStar.Int.Cast.uint8_to_uint32 (key_len a)
+
+
+/// https://tools.ietf.org/html/draft-ietf-quic-tls-23#section-5
+///
+/// We perform the three key derivations (AEAD key; AEAD iv; header protection
+/// key) when ``create`` is called. We thus store the original traffic secret
+/// only ghostly.
+///
+/// We retain the AEAD state, in order to perform the packet payload encryption.
+///
+/// We retain the Cipher state, in order to compute the mask for header protection.
+noeq
+type state_s (i: index) =
+  | State:
+      the_hash_alg:ha { the_hash_alg == i.hash_alg } ->
+      the_aead_alg:ea { the_aead_alg == i.aead_alg } ->
+      traffic_secret:G.erased (Spec.Hash.Definitions.bytes_hash the_hash_alg) ->
+      initial_pn:G.erased PN.packet_number_t ->
+      aead_state:EverCrypt.AEAD.state the_aead_alg ->
+      iv:EverCrypt.AEAD.iv_p the_aead_alg { B.length iv == 12 } ->
+      hp_key:B.buffer Secret.uint8 { B.length hp_key = QUIC.Spec.ae_keysize the_aead_alg } ->
+      pn:B.pointer PN.packet_number_t ->
+      ctr_state:CTR.state (as_cipher_alg the_aead_alg) ->
+      state_s i
+
+let footprint_s #i h s =
+  let open LowStar.Buffer in
+  AEAD.footprint h (State?.aead_state s) `loc_union`
+  CTR.footprint h (State?.ctr_state s) `loc_union`
+  loc_buffer (State?.iv s) `loc_union`
+  loc_buffer (State?.hp_key s) `loc_union`
+  loc_buffer (State?.pn s)
+
+let g_traffic_secret #i s =
+  // Automatic reveal insertion doesn't work here
+  G.reveal (State?.traffic_secret s)
+
+let g_initial_packet_number #i s =
+  // New style: automatic insertion of reveal
+  State?.initial_pn s
+
+let invariant_s #i h s =
+  let open QUIC.Spec in
+  let State hash_alg aead_alg traffic_secret initial_pn aead_state iv hp_key pn ctr_state =
+    s in
+  hash_is_keysized s; (
+  AEAD.invariant h aead_state /\
+  not (B.g_is_null aead_state) /\
+  CTR.invariant h ctr_state /\
+  not (B.g_is_null ctr_state) /\
+  B.(all_live h [ buf iv; buf hp_key; buf pn ])  /\
+  B.(all_disjoint [ CTR.footprint h ctr_state;
+    AEAD.footprint h aead_state; loc_buffer iv; loc_buffer hp_key; loc_buffer pn ]) /\
+  // : automatic insertion of reveal does not work here
+  Secret.v initial_pn <= Secret.v (B.deref h pn) /\
+  AEAD.as_kv (B.deref h aead_state) ==
+    derive_secret i.hash_alg (G.reveal traffic_secret) label_key (Spec.Agile.AEAD.key_length aead_alg) /\
+  (B.as_seq h iv) ==
+    derive_secret i.hash_alg (G.reveal traffic_secret) label_iv 12 /\
+  B.as_seq h hp_key ==
+    derive_secret i.hash_alg (G.reveal traffic_secret) label_hp (QUIC.Spec.ae_keysize aead_alg)
+  )
+
+let invariant_loc_in_footprint #_ _ _ = ()
+
+let g_last_packet_number #i s h =
+  B.deref h (State?.pn s)
+
+let frame_invariant #i l s h0 h1 =
+  AEAD.frame_invariant l (State?.aead_state (B.deref h0 s)) h0 h1;
+  CTR.frame_invariant l (State?.ctr_state (B.deref h0 s)) h0 h1
+
+let aead_alg_of_state #i s =
+  let State _ the_aead_alg _ _ _ _ _ _ _ = !*s in
+  the_aead_alg
+
+let hash_alg_of_state #i s =
+  let open FStar.HyperStack.ST in (* for the !* notation *)
+  let State the_hash_alg _ _ _ _ _ _ _ _ = !*s in
+  the_hash_alg
+
+let last_packet_number_of_state #i s =
+  let State _ _ _ _ _ _ _ pn _ = !*s in
+  !*pn
+
+
+/// For functions that perform allocations, or even functions that need
+/// temporary state, a style we adopt here is to write the core (i.e. what would
+/// normally go in-between push and pop frame) as a separate function. If
+/// needed, the core of the function takes its temporary allocations as
+/// parameters, and reasons abstractly against a region where the temporary
+/// allocations live. This gives significantly better proof performance.
+///
+/// Another bit of style: after every stateful operation, we restore manually:
+/// the modifies clause (going directly for the one we want); the invariant; the
+/// footprint preservation; then the functional correctness propertise we are
+/// seeking.
+
+val create_in_core:
+  i:index ->
+  r:HS.rid ->
+  dst: B.pointer (B.pointer_or_null (state_s i)) ->
+  initial_pn:PN.packet_number_t ->
+  traffic_secret:B.buffer Secret.uint8 {
+    B.length traffic_secret = Spec.Hash.Definitions.hash_length i.hash_alg
+  } ->
+  aead_state:AEAD.state i.aead_alg ->
+  ctr_state:CTR.state (as_cipher_alg i.aead_alg) ->
+  HST.ST unit
+    (requires fun h0 ->
+      Lemmas.hash_is_keysized_ i.hash_alg; (
+      HST.is_eternal_region r /\
+      B.live h0 dst /\ B.live h0 traffic_secret /\
+      B.(all_disjoint [ AEAD.footprint h0 aead_state; CTR.footprint h0 ctr_state;
+        loc_buffer dst; loc_buffer traffic_secret ]) /\
+      B.(loc_includes (loc_region_only true r) (AEAD.footprint h0 aead_state)) /\
+      B.(loc_includes (loc_region_only true r) (CTR.footprint h0 ctr_state)) /\
+
+      // Whatever from the invariant ought to be established already.
+      AEAD.invariant h0 aead_state /\
+      not (B.g_is_null aead_state) /\
+      CTR.invariant h0 ctr_state /\
+      not (B.g_is_null ctr_state) /\
+      AEAD.as_kv (B.deref h0 aead_state) ==
+        QUIC.Spec.(derive_secret i.hash_alg (B.as_seq h0 traffic_secret) label_key
+          (Spec.Agile.AEAD.key_length i.aead_alg))))
+    (ensures (fun h0 _ h1 ->
+      let s = B.deref h1 dst in
+      not (B.g_is_null s) /\
+      invariant h1 s /\
+
+      B.(modifies (loc_buffer dst) h0 h1) /\ (
+      let State _ _ _ initial_pn' aead_state' iv' hp_key' pn' ctr_state' = B.deref h1 s in
+      aead_state' == aead_state /\
+      ctr_state' == ctr_state /\
+      B.(fresh_loc (loc_buffer iv') h0 h1) /\
+      B.(fresh_loc (loc_buffer hp_key') h0 h1) /\
+      B.(fresh_loc (loc_buffer pn') h0 h1) /\
+      B.(fresh_loc (loc_addr_of_buffer s) h0 h1) /\
+
+      g_traffic_secret (B.deref h1 s) == B.as_seq h0 traffic_secret /\ 
+      g_last_packet_number (B.deref h1 s) h1 == initial_pn /\
+
+      G.reveal initial_pn' == initial_pn)))
+
+#push-options "--z3rlimit 50"
+let create_in_core i r dst initial_pn traffic_secret aead_state ctr_state =
+  LowStar.ImmutableBuffer.recall Impl.label_key;
+  LowStar.ImmutableBuffer.recall_contents Impl.label_key Spec.label_key;
+  LowStar.ImmutableBuffer.recall Impl.label_iv;
+  LowStar.ImmutableBuffer.recall_contents Impl.label_iv Spec.label_iv;
+  LowStar.ImmutableBuffer.recall Impl.label_hp;
+  LowStar.ImmutableBuffer.recall_contents Impl.label_hp Spec.label_hp;
+
+  (**) let h0 = HST.get () in
+  (**) assert_norm FStar.Mul.(8 * 12 <= pow2 64 - 1);
+
+  // The modifies clauses that we will transitively carry across this function body.
+  let mloc = G.hide (B.(loc_buffer dst `loc_union` loc_unused_in h0)) in
+  let e_traffic_secret: G.erased (Spec.Hash.Definitions.bytes_hash i.hash_alg) =
+    G.hide (B.as_seq h0 traffic_secret) in
+  let e_initial_pn: G.erased PN.packet_number_t = G.hide (initial_pn) in
+
+  let iv = B.malloc r (Secret.to_u8 0uy) 12ul in
+  let hp_key = B.malloc r (Secret.to_u8 0uy) (key_len32 i.aead_alg) in
+  let pn = B.malloc r initial_pn 1ul in
+  (**) let h1 = HST.get () in
+  (**) B.(modifies_loc_includes (G.reveal mloc) h0 h1 loc_none);
+  (**) assert (B.length hp_key = QUIC.Spec.ae_keysize i.aead_alg);
+
+  let s: state_s i = State #i
+    i.hash_alg i.aead_alg e_traffic_secret e_initial_pn
+    aead_state iv hp_key pn ctr_state
+  in
+
+  let s:B.pointer_or_null (state_s i) = B.malloc r s 1ul in
+  (**) let h2 = HST.get () in
+  (**) B.(modifies_loc_includes (G.reveal mloc) h1 h2 loc_none);
+  (**) B.(modifies_trans (G.reveal mloc) h0 h1 (G.reveal mloc) h2);
+
+  Impl.derive_secret i.hash_alg iv 12uy traffic_secret Impl.label_iv 2uy;
+  (**) let h3 = HST.get () in
+  (**) B.(modifies_loc_includes (G.reveal mloc) h2 h3 (loc_buffer iv));
+  (**) B.(modifies_trans (G.reveal mloc) h0 h2 (G.reveal mloc) h3);
+
+  Impl.derive_secret i.hash_alg hp_key (key_len i.aead_alg) traffic_secret Impl.label_hp 2uy;
+  (**) let h4 = HST.get () in
+  (**) B.(modifies_loc_includes (G.reveal mloc) h3 h4 (loc_buffer hp_key));
+  (**) B.(modifies_trans (G.reveal mloc) h0 h3 (G.reveal mloc) h4);
+
+  dst *= s;
+  (**) let h5 = HST.get () in
+  (**) B.(modifies_loc_includes (G.reveal mloc) h4 h5 (loc_buffer dst));
+  (**) B.(modifies_trans (G.reveal mloc) h0 h4 (G.reveal mloc) h5);
+  (**) B.(modifies_only_not_unused_in (loc_buffer dst) h0 h5)
+#pop-options
+
+#push-options "--z3rlimit 256"
+let create_in i r dst initial_pn traffic_secret =
+  LowStar.ImmutableBuffer.recall Impl.label_key;
+  LowStar.ImmutableBuffer.recall_contents Impl.label_key Spec.label_key;
+
+  (**) let h0 = HST.get () in
+
+  HST.push_frame ();
+  (**) let h1 = HST.get () in
+  let mloc = G.hide (B.(loc_region_only true (HS.get_tip h1) `loc_union` loc_buffer dst
+    `loc_union` loc_unused_in h0)) in
+
+  let aead_key = B.alloca (Secret.to_u8 0uy) (key_len32 i.aead_alg) in
+  let aead_state: B.pointer (B.pointer_or_null (AEAD.state_s i.aead_alg)) =
+    B.alloca B.null 1ul in
+  let ctr_state: B.pointer (B.pointer_or_null (CTR.state_s (as_cipher_alg i.aead_alg))) =
+    B.alloca (B.null #(CTR.state_s (as_cipher_alg i.aead_alg))) 1ul in
+  let dummy_iv = B.alloca (Secret.to_u8 0uy) 12ul in
+
+  (**) let h2 = HST.get () in
+  (**) B.(modifies_loc_includes (G.reveal mloc) h1 h2 (loc_none));
+
+  Impl.derive_secret i.hash_alg aead_key (key_len i.aead_alg) traffic_secret Impl.label_key 3uy;
+  (**) let h3 = HST.get () in
+  (**) B.(modifies_loc_includes (G.reveal mloc) h2 h3 (loc_buffer aead_key));
+  (**) B.(modifies_trans (G.reveal mloc) h1 h2 (G.reveal mloc) h3);
+
+  let ret = AEAD.create_in #i.aead_alg r aead_state aead_key in
+  (**) let h4 = HST.get () in
+  (**) B.(modifies_loc_includes (G.reveal mloc) h3 h4 (loc_buffer aead_state));
+  (**) B.(modifies_trans (G.reveal mloc) h1 h3 (G.reveal mloc) h4);
+
+  let ret' = CTR.create_in (as_cipher_alg i.aead_alg) r ctr_state aead_key dummy_iv 12ul 0ul in
+  (**) let h5 = HST.get () in
+  (**) B.(modifies_loc_includes (G.reveal mloc) h4 h5 (loc_buffer ctr_state));
+  (**) B.(modifies_trans (G.reveal mloc) h1 h4 (G.reveal mloc) h5);
+  (**) B.(modifies_only_not_unused_in B.(loc_region_only true (HS.get_tip h1) `loc_union` loc_buffer dst) h1 h5);
+
+  match ret with
+  | UnsupportedAlgorithm ->
+      HST.pop_frame ();
+      (**) let h6 = HST.get () in
+      (**) B.(modifies_fresh_frame_popped h0 h1 (loc_buffer dst) h5 h6);
+      UnsupportedAlgorithm
+
+  | Success ->
+
+  match ret' with
+  | UnsupportedAlgorithm ->
+      HST.pop_frame ();
+      (**) let h6 = HST.get () in
+      (**) B.(modifies_fresh_frame_popped h0 h1 (loc_buffer dst) h5 h6);
+      UnsupportedAlgorithm
+
+  | Success ->
+
+      let aead_state: AEAD.state i.aead_alg = !*aead_state in
+      (**) assert (AEAD.invariant h5 aead_state);
+
+      let ctr_state: CTR.state (as_cipher_alg i.aead_alg) = !*ctr_state in
+      (**) assert (CTR.invariant h5 ctr_state);
+
+      create_in_core i r dst initial_pn traffic_secret aead_state ctr_state;
+      (**) let h6 = HST.get () in
+
+      (**) B.(modifies_loc_includes
+        (loc_region_only true (HS.get_tip h1) `loc_union` loc_buffer dst) h5 h6
+        (loc_buffer dst));
+      (**) B.(modifies_trans
+        (loc_region_only true (HS.get_tip h1) `loc_union` loc_buffer dst)
+        h1 h5
+        (loc_region_only true (HS.get_tip h1) `loc_union` loc_buffer dst)
+        h6);
+
+      HST.pop_frame ();
+      (**) let h7 = HST.get () in
+      (**) B.(modifies_fresh_frame_popped h0 h1 (loc_buffer dst) h6 h7);
+      (**) frame_invariant (B.loc_region_only false (HS.get_tip h6)) (B.deref h7 dst) h6 h7;
+
+      Success
+#pop-options
+
+#push-options "--z3rlimit 64"
+
+let encrypt
+  #i s dst dst_pn h plain plain_len
+=
+  let m0 = HST.get () in
+  let State hash_alg aead_alg e_traffic_secret e_initial_pn
+    aead_state iv hp_key bpn ctr_state = !*s
+  in
+  let last_pn = !* bpn in
+  let pn = last_pn `Secret.add` Secret.to_u64 1uL in
+  B.upd bpn 0ul pn;
+  B.upd dst_pn 0ul pn;
+  let m1 = HST.get () in
+  assert (B.modifies (footprint m0 s `B.loc_union` B.loc_buffer dst_pn) m0 m1);
+  frame_header h pn  (footprint m0 s `B.loc_union` B.loc_buffer dst_pn) m0 m1;
+  Impl.encrypt aead_alg aead_state iv ctr_state hp_key dst h pn plain (Secret.to_u32 plain_len)
+
+#pop-options
+
+
+/// Initial secrets
+/// ---------------
+
+// TODO: these three should be immutable buffers but we don't have const
+// pointers yet for HKDF.
+#push-options "--warn_error -272"
+let initial_salt: initial_salt:B.buffer U8.t {
+  B.length initial_salt = 20 /\
+  B.recallable initial_salt
+} =
+  [@inline_let]
+  let l = [
+    0xc3uy; 0xeeuy; 0xf7uy; 0x12uy; 0xc7uy; 0x2euy; 0xbbuy; 0x5auy;
+    0x11uy; 0xa7uy; 0xd2uy; 0x43uy; 0x2buy; 0xb4uy; 0x63uy; 0x65uy;
+    0xbeuy; 0xf9uy; 0xf5uy; 0x02uy
+  ] in
+  assert_norm (List.Tot.length l = 20);
+  B.gcmalloc_of_list HS.root l
+
+let server_in: server_in:B.buffer U8.t {
+  B.length server_in = 9 /\
+  B.recallable server_in
+} =
+  [@inline_let]
+  let l = [
+    0x73uy; 0x65uy; 0x72uy; 0x76uy; 0x65uy; 0x72uy; 0x20uy; 0x69uy; 0x6euy
+  ] in
+  assert_norm (List.Tot.length l = 9);
+  B.gcmalloc_of_list HS.root l
+
+let client_in: client_in:B.buffer U8.t {
+  B.length client_in = 9 /\
+  B.recallable client_in
+} =
+  [@inline_let]
+  let l = [
+    0x63uy; 0x6cuy; 0x69uy; 0x65uy; 0x6euy; 0x74uy; 0x20uy; 0x69uy; 0x6euy
+  ] in
+  assert_norm (List.Tot.length l = 9);
+  B.gcmalloc_of_list HS.root l
+#pop-options
+
+#push-options "--z3rlimit 64"
+
+let initial_secrets dst_client dst_server cid cid_len =
+  (**) let h0 = HST.get () in
+  (**) B.recall initial_salt;
+  (**) B.recall server_in;
+  (**) B.recall client_in;
+  assert_norm (Spec.Agile.Hash.(hash_length SHA2_256) = 32);
+
+  HST.push_frame ();
+  (**) let h1 = HST.get () in
+  (**) let mloc = G.hide (B.(loc_buffer dst_client `loc_union`
+    loc_buffer dst_server `loc_union` loc_region_only true (HS.get_tip h1))) in
+
+  B.loc_unused_in_not_unused_in_disjoint h1;
+  let secret = B.alloca (Secret.to_u8 0uy) 32ul in
+  
+  (* we allocate a temporary buffer to copy the initial_salt,
+     server_in and client_in and then to hide it through
+     SecretBuffer.with_whole_buffer_hide_weak_modifies, because if we
+     directly hide those global buffers, then we won't be able to
+     prove that the livenesses of function arguments are preserved,
+     because they are not disjoint from the global buffers.  *)
+
+  let h15 = HST.get () in
+  B.loc_unused_in_not_unused_in_disjoint h15;
+  let tmp = B.alloca 0uy 20ul in
+  B.blit initial_salt 0ul tmp 0ul 20ul;
+  
+  (**) let h2 = HST.get () in
+
+  (**) Lemmas.hash_is_keysized_ Spec.Agile.Hash.SHA2_256;
+  let h25 = HST.get () in
+  SecretBuffer.with_whole_buffer_hide_weak_modifies
+    tmp
+    h25
+    (B.loc_buffer secret `B.loc_union` B.loc_buffer cid)
+    (B.loc_buffer secret)
+    false
+    (fun _ _ m -> True)
+    (fun _ bs ->
+      EverCrypt.HKDF.extract Spec.Agile.Hash.SHA2_256 secret bs 20ul
+        cid cid_len
+    );
+  (**) let h3 = HST.get () in
+  (**) B.(modifies_trans (G.reveal mloc) h1 h2 (G.reveal mloc) h3);
+
+  let tmp_client_in = B.sub tmp 0ul 9ul in
+  B.blit client_in 0ul tmp_client_in 0ul 9ul;
+  let h35 = HST.get () in
+  SecretBuffer.with_whole_buffer_hide_weak_modifies
+    tmp_client_in
+    h35
+    (B.loc_buffer secret `B.loc_union` B.loc_buffer dst_client)
+    (B.loc_buffer dst_client)
+    false
+    (fun _ _ m -> True)
+    (fun _ bs ->
+      EverCrypt.HKDF.expand Spec.Agile.Hash.SHA2_256 dst_client secret 32ul bs 9ul 32ul
+    );
+  (**) let h4 = HST.get () in
+  (**) B.(modifies_trans (G.reveal mloc) h1 h3 (G.reveal mloc) h4);
+
+  let tmp_server_in = B.sub tmp 0ul 9ul in
+  B.blit server_in 0ul tmp_server_in 0ul 9ul;
+  let h45 = HST.get () in
+  SecretBuffer.with_whole_buffer_hide_weak_modifies
+    tmp_server_in
+    h45
+    (B.loc_buffer secret `B.loc_union` B.loc_buffer dst_server)
+    (B.loc_buffer dst_server)
+    false
+    (fun _ _ m -> True)
+    (fun _ bs ->
+      EverCrypt.HKDF.expand Spec.Agile.Hash.SHA2_256 dst_server secret 32ul bs 9ul 32ul
+    );
+  (**) let h5 = HST.get () in
+  (**) B.(modifies_trans (G.reveal mloc) h1 h4 (G.reveal mloc) h5);
+
+  HST.pop_frame ();
+  (**) let h6 = HST.get () in
+  (**) B.modifies_fresh_frame_popped h0 h1
+  (**)   B.(loc_buffer dst_client `loc_union` loc_buffer dst_server) h5 h6
+
+#restart-solver
+
+
+#push-options "--z3rlimit 128"
+
+let decrypt
+  #i s dst packet len cid_len
+=
+  let m0 = HST.get () in
+  let State hash_alg aead_alg e_traffic_secret e_initial_pn
+    aead_state iv hp_key bpn ctr_state = !*s
+  in
+  let last_pn = !* bpn in
+  let res = Impl.decrypt aead_alg aead_state iv ctr_state hp_key packet len dst last_pn (FStar.Int.Cast.uint8_to_uint32 cid_len) in
+  let m1 = HST.get () in
+  if res = Success
+  then begin
+    let r = B.index dst 0ul in
+    let pn = r.Base.pn in
+    let pn' = Secret.max64 last_pn pn in
+    B.upd bpn 0ul pn';
+    let m2 = HST.get () in
+    assert (B.modifies (footprint m0 s) m1 m2);
+    frame_header r.header pn  (footprint m0 s) m1 m2;
+    assert (
+      let k = derive_k i s m0 in
+      let iv = derive_iv i s m0 in
+      let pne = derive_pne i s m0 in
+      match Spec.decrypt i.aead_alg k iv pne (Secret.v last_pn) (U8.v cid_len) (B.as_seq m0 packet) with
+      | Spec.Success gh plain rem ->
+        B.as_seq m1 (B.gsub packet (Secret.reveal r.header_len) (Secret.reveal r.plain_len)) == plain
+      | _ -> False
+    )
+  end;
+  res
+
+#pop-options
